port examples to NotationsCustomEntry

bedrock2/src/bedrock2Examples/ARPResponder.v
@@ -6,9 +6,8 @@ Section WithParameters.
   Context {p : FE310CSemantics.parameters}.
   Import Syntax BinInt String List.ListNotations ZArith.
   Local Open Scope string_scope. Local Open Scope Z_scope. Local Open Scope list_scope.
-  Local Coercion literal (z : Z) : expr := expr.literal z.
-  Local Coercion var (x : String.string) : expr := expr.var x.
-  Local Definition bedrock_func : Type := function.
+  Local Coercion expr.literal : Z >-> expr.
+  Local Coercion expr.var : String.string >-> expr.
   Local Coercion name_of_func (f : function) : String.string := fst f.
 
 Definition arp : bedrock_func :=
@@ -89,7 +88,7 @@ Definition ethernet : bedrock_func :=
     let ethertype : String.string := "ethertype" in
   ("ethernet", ((buf::len::nil), @nil String.string, bedrock_func_body:(
     require (constr:(14) < len) else { /*skip*/ } ;
-    ethertype = ((load1(buf + constr:(12)) << constr:(8)) | (load1(buf + constr:(13))));
+    ethertype = (load1(buf + constr:(12)) << constr:(8)) | (load1(buf + constr:(13)));
     require (constr:(Ox"600"-1) < ethertype) else { /*skip*/ };
     if (ethertype == constr:(Ox"0800")) {
       ipv4(buf+constr:(14), len-constr:(14))
@@ -98,14 +97,13 @@ Definition ethernet : bedrock_func :=
     }
 ))).
 
-(*
-Require Import bedrock2.Bytedump bedrock2.Byte bedrock2.ToCString.
-Local Open Scope bytedump_scope.
+Require Import bedrock2.ToCString.
 Goal True.
-  let c_code := eval cbv in (of_string (c_module (ethernet::arp::ipv4::nil))) in
+  let c_code := eval cbv in ((c_module (ethernet::arp::ipv4::nil))) in
       idtac
-        (* c_code *)
+        (*
+        c_code
+        *)
   .
 Abort.
-*)
 End WithParameters.
