bedrock2/src/bedrock2Examples/Demos.v
@@ -1,181 +1,91 @@
 Require Import Coq.Lists.List. Import ListNotations.
 Require Import coqutil.Macros.subst coqutil.Macros.unique bedrock2.Syntax.
-Require bedrock2.NotationsInConstr.
+Require Import bedrock2.NotationsCustomEntry.
 Require Import coqutil.sanity.
 
-Import BinInt String.
 Local Open Scope string_scope. Local Open Scope Z_scope. Local Open Scope list_scope.
+Import BinInt String.
+Local Coercion expr.literal : Z >-> expr.
+Local Coercion expr.var : String.string >-> expr.
+Local Coercion name_of_func (f : function) : String.string := fst f.
 
-(* Boilerplate to get variable names.
-   The names are in separate modules to allow the same variable name to be used in several
-   programs defined in the same file. *)
+Definition bsearch: func :=
+  let left := "left" in let right := "right" in let target := "target" in let mid := "mid" in
+  ("bsearch", ([left; right; target], [left], bedrock_func_body:(
+  while (right - left) {
+    mid = left + (((right-left) >> constr:(4)) << constr:(3));
+    if (load(mid) < target) {
+      left = mid + constr:(8)
+    } else {
+      right = mid
+    };
+    constr:(cmd.unset mid)
+  }
+))).
 
-Module BinarySearch.
-  Class Names := {
-    left : String.string;
-    right : String.string;
-    target : String.string;
-    mid : String.string;
-    tmp : String.string;
-  }.
-  Module StringNames.
-    Instance Inst: Names := {
-      left := "left";
-      right := "right";
-      target := "target";
-      mid := "mid";
-      tmp := "tmp";
-    }.
-  End StringNames.
-End BinarySearch.
+(* input_base is an address fixed at compile time *)
+Definition listsum(input_base: Z): func :=
+  let sumreg := "sumreg" in let n := "n" in let i := "i" in let a := "a" in
+  ("listsum", ([], [sumreg], bedrock_func_body:(
+  sumreg = constr:(0);
+  n = load4(input_base);
+  i = constr:(0);
+  while (i < n) {
+    a = load4(constr:(input_base + 4) + (i << constr:(2)));
+    sumreg = sumreg + a;
+    i = i + constr:(1)
+  }
+))).
 
-Module ListSum.
-  Class Names := {
-    n: String.string;
-    i: String.string;
-    sumreg: String.string;
-    a: String.string;
-  }.
-  Module StringNames.
-    Instance Inst: Names := {
-      n := "n";
-      i := "i";
-      sumreg := "sumreg";
-      a := "a";
-    }.
-  End StringNames.
-End ListSum.
+(* input_base is an address fixed at compile time *)
+Definition fibonacci(n: Z): func :=
+  let a := "a" in let b := "b" in let i := "i" in let n := "n" in let c := "c" in
+  ("fibonacci", ([], [b], bedrock_func_body:(
+  a = constr:(0);
+  b = constr:(1);
+  i = constr:(0);
+  while (i < n) {
+    c = a + b;
+    a = b;
+    b = c;
+    i = i + constr:(1)
+  }
+))).
 
-Module Fibonacci.
-  Class Names := {
-    a: String.string;
-    b: String.string;
-    c: String.string;
-    i: String.string;
-  }.
-  Module StringNames.
-    Instance Inst: Names := {
-      a := "a";
-      b := "b";
-      c := "c";
-      i := "i";
-    }.
-  End StringNames.
-End Fibonacci.
+Definition fibonacciServer (n_load_addr n_store_addr: Z): func :=
+  let b := "b" in let n := "n" in let a := "a" in let i := "i" in let c := "c" in
+  ("fibonacciserver", ([], [b], bedrock_func_body:(
+  n = load4(n_load_addr);
+  a = constr:(0);
+  b = constr:(1);
+  i = constr:(0);
+  if (n < constr:(47)) {
+    while (i < n) {
+      c = a + b;
+      a = b;
+      b = c;
+      i = i + constr:(1)
+    }
+  } else {
+    b = constr:(-1)
+  };
+  store4(n_store_addr, b)
+))).
 
+Definition dummy: func := ("dummy", ([], [], cmd.skip)).
 
-Module FibonacciServer.
-  Class Names := {
-    a: String.string;
-    b: String.string;
-    c: String.string;
-    i: String.string;
-    n: String.string;
-  }.
-  Module StringNames.
-    Instance Inst: Names := {
-      a := "a";
-      b := "b";
-      c := "c";
-      i := "i";
-      n := "n";
-    }.
-  End StringNames.
-End FibonacciServer.
+Definition allProgs: list func :=
+  Eval unfold bsearch, listsum, fibonacci in
+    [bsearch; listsum 1024; fibonacci 6].
 
-Section Demos.
-
-  Local Coercion var(x : String.string): expr.expr := expr.var x.
-  Local Coercion literal (z : Z) : expr := expr.literal z.
-
-  Import bedrock2.NotationsInConstr.
-  Import BinarySearch.
-  Definition bsearch: func := ("bsearch", ([left; right; target], [left], bedrock_func_body:(
-    while (right - left) {{
-      mid = left + (((right-left) >> 4) << 3);;
-      if ((expr.load access_size.word mid) < target) {{
-        left = mid + 8
-      }} else {{
-        right = mid
-      }};;
-      cmd.unset mid
-    }}
-  ))).
-
-  Import ListSum.
-  (* input_base is an address fixed at compile time *)
-  Definition listsum(input_base: Z): func := ("listsum", ([], [sumreg], bedrock_func_body:(
-    sumreg = 0;;
-    n = *(uint32_t*) input_base;;
-    i = 0;;
-    while (i < n) {{
-      a = *(uint32_t*) ((input_base + 4)%Z + (i << 2));;
-      sumreg = sumreg + a;;
-      i = i + 1
-    }}
-  ))).
-
-  Import Fibonacci.
-  (* input_base is an address fixed at compile time *)
-  Definition fibonacci(n: Z): func := ("fibonacci", ([], [b], bedrock_func_body:(
-    a = 0;;
-    b = 1;;
-    i = 0;;
-    while (i < n) {{
-      c = a + b;;
-      a = b;;
-      b = c;;
-      i = i + 1
-    }}
-  ))).
-
-  Import FibonacciServer.
-  Definition fibonacciServer (n_load_addr n_store_addr: Z): func := ("fibonacciserver", ([], [b], bedrock_func_body:(
-    n = *(uint32_t*) n_load_addr;;
-    a = 0;;
-    b = 1;;
-    i = 0;;
-    if (n < 47) {{
-      while (i < n) {{
-        c = a + b;;
-        a = b;;
-        b = c;;
-        i = i + 1
-      }}
-    }} else {{
-      b = -1
-    }};;
-    *(uint32_t*) n_store_addr = b
-  ))).
-
-  Definition dummy: func := ("dummy", ([], [], cmd.skip)).
-
-  Definition allProgs: list func :=
-    Eval unfold bsearch, listsum, fibonacci in
-      [bsearch; listsum 1024; fibonacci 6].
-
-  (*Print allProgs.*)
-
-  Definition prog(name: string): func :=
-    match find (fun '(n, _) => if string_dec n name then true else false) allProgs with
-    | Some p => p
-    | None => dummy
-    end.
-
-End Demos.
-
-(* let's print them again in AST form: *)
-(* Print allProgs. *)
+(*
+Print allProgs.
+*)
 
 Require Import bedrock2.ToCString.
-Definition allProgsAsCString: string :=
+Definition allProgsAsCString : string :=
   Eval cbv in c_module allProgs.
 
 (*
 Print allProgsAsCString.
 *)
-
-Definition allProgsE :=
-  Eval cbv in allProgs.
-
-(* Print allProgsE. *)
